# HW Review

Class: Physics
Created: Oct 15, 2020 11:40 AM
Type: Notes

### Q3

$e^{-2\pi i/4 }(z+1)=f(z)$

$f(0)=e^{-2\pi i/4}$

Add up all steps and take magnitude

$$1+1e^{-2\pi i/9}+1e^{-4\pi i/9}+1e^{-6\pi i/9}\\a=1 r e^{-2\pi i/9}\\S_n=\frac{a(1-r^n)}{1-r}\\S_4=\frac{1-(e^{-2\pi i/9})^4}{1-e^{-2\pi i/9}}$$

$$\frac{|1-e^{-8\pi i/9}|}{|1-e^{-2\pi i/9}|}=\frac{|1-(\cos{8\pi /9}-i\sin{8\pi /9})|}{|1-(\cos{2\pi /9}-i\sin{2\pi /9})|}=\frac{1-2\cos{8\pi /9}+\cos^2{8\pi /9}+\sin^2{8\pi /9}}{1-2\cos{2\pi /9}+\cos^2{2\pi /9}+\sin^2{2\pi /9}}$$

$$\frac{2-2\cos{8\pi/9}}{2-2\cos{2\pi/9}}=z^2_4\\z_4=\frac{\sin{4\pi/9}}{\sin{\pi/9}}$$

### Q8

![[HW Review/Untitled.png]]

![[HW Review/Untitled 1.png]]
